Semantics: Environment: added environment definition.
Environment (also, valuation) is a function from the set of all
variables to the domain of a first-order structure.

Defined extensions of environment to terms and vectors. Tried to prove
a lemma from Brotherstons PhD thesis, but got stuck in the inductive
case. Do I need an even better induction principle, or should I learn
about induction and destruction of dependent types better?

Structure.v
@@ -1,23 +1,75 @@
 Require Coq.Unicode.Utf8.
 Require Coq.Vectors.Vector.
+Require Import Arith Bool.
+Require Import FunctionalExtensionality.
+Require Import Sets.Ensembles.
 Require Import CFOLID.Signature.
-
-Definition vec := Vector.t.
+Require Import CFOLID.Term.
 
 Section structure.
   Variable Σ : signature.
 
-  Structure structure := {      (* struktura *)
-      domain : Type;            (* nosač *)
+  Structure structure := {
+      domain : Type;
       interpF : forall f : FuncS Σ, vec domain (FuncArr f) -> domain;
       interpP : forall P : PredS Σ, vec domain (PredArr P) -> Prop;
       interpIP : forall P : IndPredS Σ, vec domain (IndPredArr P) -> Prop;
     }.
 End structure.
 
-Arguments structure {Σ}.
 Arguments domain {Σ}.
 Arguments interpF {Σ}.
 Arguments interpP {Σ}.
 Arguments interpIP {Σ}.
 Notation "| M |" := (domain M) (no associativity, at level 150).
+
+Section environment.
+  Variable Σ : signature.
+  Variable M : structure Σ.
+
+  Definition env_var := var -> |M|.
+
+  Definition env_var_subst (ρ : env_var) (x : var) (d : |M|)
+    : var -> |M| :=
+    fun (y : var) => if y =? x then d else ρ y.
+
+  Section extended_environment.
+    Variable ρvar : env_var.
+              
+    Fixpoint env (t : term Σ) : |M| :=
+      match t with
+      | TVar x => ρvar x
+      | TFunc f args => interpF M f (Vector.map env args)
+      end.
+
+    Definition env_vec n (v : vec (term Σ) n) : vec (|M|) n :=
+      Vector.map env v.
+
+    Fixpoint env_subst (t : term Σ) (x : var) (d : |M|) : |M| :=
+      match t with
+      | TVar y => env_var_subst ρvar x d y
+      | TFunc f args => interpF M f (Vector.map (fun st => env_subst st x d) args)
+      end.
+  End extended_environment.
+
+  Section lemma_2_1_5.
+    Variable ρvar : env_var.
+    Definition ρ := env ρvar.
+
+    Lemma env_subst_sanity1 : forall (t : term Σ) (x : var) (d : |M|),
+        ~ In _ (Var t) x -> env_subst ρvar t x d = env ρvar t.
+    Proof.
+      intros t; induction t as [v | f args IH] using term_better_ind;
+        intros x d x_not_in_t.
+      - simpl; unfold env_var_subst; destruct (v =? x) eqn:eq_vx.
+        + exfalso. apply x_not_in_t. rewrite Nat.eqb_eq in eq_vx; subst.
+          constructor.
+        + reflexivity.
+      - simpl. f_equal. inversion IH; subst.
+        + reflexivity.
+        + admit.
+          (* TODO this is a big mess because of Vector  *)
+    Admitted.
+                      
+  End lemma_2_1_5.
+End environment.
